src/cbor/CBOR.SteelST.fst
@@ -571,3 +571,326 @@ let jump_raw_data_item
 = fun a ->
     let sq = Steel.ST.HigherArray.intro_fits_u64 () in
     jump_raw_data_item' sq a
+
+(* 4.2 Ordering of map keys *)
+
+module NL = LowParse.SteelST.VCList.Sorted
+module SB = LowParse.SteelST.SeqBytes
+
+inline_for_extraction
+noextract
+let map_entry_order_impl
+  (#kkey: Ghost.erased parser_kind)
+  (#key: Type0)
+  (pkey: parser kkey key)
+  (#key_order: Ghost.erased (key -> key -> bool))
+  (key_order_impl: NL.order_impl pkey key_order)
+  (#kvalue: Ghost.erased parser_kind)
+  (#value: Type0)
+  (pvalue: parser kvalue value)
+: Pure (NL.order_impl (pkey `nondep_then` pvalue) (map_entry_order key_order value))
+    (requires (kkey.parser_kind_subkind == Some ParserStrong))
+    (ensures (fun _ -> True))
+= fun #va1 #va2 a1 a2 ->
+    let av1 = g_split_pair pkey pvalue a1 in
+    let _ = gen_elim () in
+    let av2 = g_split_pair pkey pvalue a2 in
+    let _ = gen_elim () in
+    let res = key_order_impl a1 a2 in
+    let _ = merge_pair pkey pvalue a1 av1 in
+    vpattern_rewrite (aparse _ a1) va1;
+    let _ = merge_pair pkey pvalue a2 av2 in
+    vpattern_rewrite (aparse _ a2) va2;
+    return res
+
+let get_major_type_synth_raw_data_item
+  (x: raw_data_item')
+: Lemma
+  (get_major_type (synth_raw_data_item x) == (match x with (| (| (major_type, _), _ |), _ |) -> major_type))
+= assert_norm (pow2 3 == 8)
+
+#push-options "--z3rlimit 16 --split_queries always"
+
+#restart-solver
+let read_major_type
+  (#va: v parse_raw_data_item_kind raw_data_item)
+  (a: byte_array)
+: ST byte
+    (aparse parse_raw_data_item a va)
+    (fun _ -> aparse parse_raw_data_item a va)
+    True
+    (fun res -> res == get_major_type va.contents)
+= Classical.forall_intro parse_raw_data_item_eq;
+  let _ = rewrite_aparse a (parse_dtuple2 parse_header (parse_content parse_raw_data_item) `parse_synth` synth_raw_data_item) in
+  let va1 = elim_synth _ _ a () in // (parse_dtuple2 parse_header (parse_content parse_raw_data_item)) synth_raw_data_item a () in
+  get_major_type_synth_raw_data_item va1.contents;
+  let a_content = ghost_split_dtuple2_full _ _ a in // parse_header (parse_content parse_raw_data_item) a in
+  let _ = gen_elim () in
+  let _ = rewrite_aparse a (parse_dtuple2 parse_initial_byte parse_long_argument) in
+  let a_long = ghost_split_dtuple2_full _ _ a in
+  let _ = gen_elim () in
+  let res = read_initial_byte a (aparse _ a_content _ `star` aparse _ a_long _) byte (fun res -> aparse parse_raw_data_item a va `star` pure (res == get_major_type va.contents)) (fun (major_type, _) ->
+    let res = major_type in
+    let _ = intro_dtuple2 parse_initial_byte parse_long_argument a a_long in
+    let _ = rewrite_aparse a parse_header in
+    let _ = intro_dtuple2 parse_header (parse_content parse_raw_data_item) a a_content in
+    noop ();
+    let _ = intro_synth (parse_dtuple2 parse_header (parse_content parse_raw_data_item)) synth_raw_data_item a () in
+    let _ = rewrite_aparse a parse_raw_data_item in
+    noop ();
+    vpattern_rewrite (aparse parse_raw_data_item a) va;
+    return res
+  )
+  in
+  let _ = elim_pure _ in
+  return res
+
+let read_argument_as_uint64
+  (#va: v parse_raw_data_item_kind raw_data_item)
+  (a: byte_array)
+: ST UInt64.t
+    (aparse parse_raw_data_item a va)
+    (fun _ -> aparse parse_raw_data_item a va)
+    True
+    (fun res ->
+      let (| (| b, x |), _ |) = synth_raw_data_item_recip va.contents in
+      res == argument_as_uint64 b x
+    )
+= Classical.forall_intro parse_raw_data_item_eq;
+  let _ = rewrite_aparse a (parse_dtuple2 parse_header (parse_content parse_raw_data_item) `parse_synth` synth_raw_data_item) in
+  let va1 = elim_synth _ _ a () in // (parse_dtuple2 parse_header (parse_content parse_raw_data_item)) synth_raw_data_item a () in
+  let a_content = ghost_split_dtuple2_full _ _ a in // parse_header (parse_content parse_raw_data_item) a in
+  let _ = gen_elim () in
+  let res = jump_header a (aparse _ a_content _) UInt64.t (fun res -> aparse parse_raw_data_item a va `star` pure (
+      let (| (| b, x |), _ |) = synth_raw_data_item_recip va.contents in
+      res == argument_as_uint64 b x
+  )) (fun _ (| b, x |) ->
+    let res = argument_as_uint64 b x in
+    let _ = intro_dtuple2 parse_header (parse_content parse_raw_data_item) a a_content in
+    noop ();
+    let _ = intro_synth (parse_dtuple2 parse_header (parse_content parse_raw_data_item)) synth_raw_data_item a () in
+    let _ = rewrite_aparse a parse_raw_data_item in
+    noop ();
+    vpattern_rewrite (aparse parse_raw_data_item a) va;
+    return res
+  )
+  in
+  let _ = elim_pure _ in
+  return res
+
+module AP = LowParse.SteelST.ArrayPtr
+
+#restart-solver
+unfold
+let get_raw_data_item_payload_map_post
+  (va: v parse_raw_data_item_kind raw_data_item)
+  (vh: v (get_parser_kind parse_header) header)
+  (n: nat)
+  (vc: v (NL.parse_nlist_kind n (and_then_kind parse_raw_data_item_kind parse_raw_data_item_kind)) (NL.nlist n (raw_data_item & raw_data_item)))
+: GTot prop
+=
+        let (| h, c |) = synth_raw_data_item_recip va.contents in
+        let (| b, x |) = h in
+        // order of the following conjuncts matters for typechecking
+        vh.contents == h /\
+        n == UInt64.v (argument_as_uint64 b x) /\
+        va.contents == Map vc.contents /\
+        vc.contents == c /\
+        AP.merge_into (array_of' vh) (array_of' vc) (array_of va)
+
+#set-options "--ide_id_info_off"
+
+let elim_synth'
+  #opened
+  #k1 #t1 (p1: parser k1 t1)
+  #t2 (f2: t1 -> GTot t2) (g1: t2 -> GTot t1)
+  #va2 (a: byte_array)
+  (sq: squash (synth_injective f2 /\
+    synth_inverse f2 g1
+  ))
+: STGhost (v k1 t1) opened
+    (aparse (p1 `parse_synth` f2) a va2)
+    (fun va -> aparse p1 a va)
+    True
+    (fun va ->
+      array_of va2 == array_of va /\
+      va2.contents == f2 (va.contents) /\
+      va.contents == g1 va2.contents
+    )
+= let va = elim_synth p1 f2 a () in
+  assert (f2 (g1 va2.contents) == va2.contents);
+  noop ();
+  va
+
+let get_raw_data_item_payload_map
+  (#opened: _)
+  (#va: v parse_raw_data_item_kind raw_data_item)
+  (a: byte_array)
+: STGhost (Ghost.erased byte_array) opened
+    (aparse parse_raw_data_item a va)
+    (fun a' -> exists_ (fun vh -> exists_ (fun (n: nat) -> exists_ (fun vc ->
+      aparse parse_header a vh `star`
+      aparse (NL.parse_nlist n (parse_raw_data_item `nondep_then` parse_raw_data_item)) a' vc `star`
+      pure (get_raw_data_item_payload_map_post va vh n vc)
+    ))))
+    (Map? va.contents)
+    (fun _ -> True)
+= Classical.forall_intro parse_raw_data_item_eq;
+  let _ = rewrite_aparse a (parse_dtuple2 parse_header (parse_content parse_raw_data_item) `parse_synth` synth_raw_data_item) in
+  let va1 = elim_synth' _ _ synth_raw_data_item_recip a () in // (parse_dtuple2 parse_header (parse_content parse_raw_data_item)) synth_raw_data_item a () in
+  let a' = ghost_split_dtuple2_full _ _ a in // parse_header (parse_content parse_raw_data_item) a in
+  let _ = gen_elim () in
+  let vh = vpattern_replace (aparse _ a) in
+  let (| b, x |) = vh.contents in
+  let n = UInt64.v (argument_as_uint64 b x) in
+  let vc = rewrite_aparse a' (NL.parse_nlist n (parse_raw_data_item `nondep_then` parse_raw_data_item)) in
+  assert (get_raw_data_item_payload_map_post va vh n vc);
+  noop ();
+  a'
+
+let intro_raw_data_item_map
+  (#opened: _)
+  (#vh: v (get_parser_kind parse_header) header)
+  (h: byte_array)
+  (#n: nat)
+  (#vc: v (NL.parse_nlist_kind n (and_then_kind parse_raw_data_item_kind parse_raw_data_item_kind)) (NL.nlist n (raw_data_item & raw_data_item)))
+  (c: byte_array)
+: STGhost (v parse_raw_data_item_kind raw_data_item) opened
+    (aparse parse_header h vh `star`
+      aparse (NL.parse_nlist n (parse_raw_data_item `nondep_then` parse_raw_data_item)) c vc
+    )
+    (fun va -> aparse parse_raw_data_item h va)
+    (
+      let (| b, x |) = vh.contents in
+      let (major_type, _) = b in
+      n == UInt64.v (argument_as_uint64 b x) /\
+      major_type == get_major_type (Map vc.contents) /\
+      AP.adjacent (array_of' vh) (array_of' vc)
+    )
+    (fun va ->
+      get_raw_data_item_payload_map_post va vh n vc
+    )
+= Classical.forall_intro parse_raw_data_item_eq;
+  let h' = uint64_as_argument (get_major_type (Map vc.contents)) (UInt64.uint_to_t n) in
+  assert (vh.contents == h');
+  noop ();
+  let _ = rewrite_aparse c (parse_content parse_raw_data_item vh.contents) in
+  let _ = intro_dtuple2 parse_header (parse_content parse_raw_data_item) h c in
+  let _ = intro_synth (parse_dtuple2 parse_header (parse_content parse_raw_data_item)) synth_raw_data_item h () in 
+  rewrite_aparse h parse_raw_data_item
+
+#restart-solver
+inline_for_extraction
+noextract
+let check_data_item_wf_head
+  (#order: Ghost.erased (raw_data_item -> raw_data_item -> bool))
+  (order_impl: NL.order_impl parse_raw_data_item order)
+  (sq: squash (SZ.fits_u64))
+: Tot (pred_recursive_base_t serialize_raw_data_item_param (data_item_wf_head order))
+= fun a va ->
+  rewrite (aparse _ a _) (aparse parse_raw_data_item a va);
+  let major_type = read_major_type a in
+  if major_type = 5uy
+  then begin
+    let n64 = read_argument_as_uint64 a in
+    let n = SZ.uint64_to_sizet n64 in
+    let gac = get_raw_data_item_payload_map a in
+    let _ = gen_elim () in
+    let ac = hop_aparse_aparse (jumper_of_read_and_jump jump_header) _ a gac in
+    let _ = rewrite_aparse ac (NL.parse_nlist (SZ.v n) (parse_raw_data_item `nondep_then` parse_raw_data_item)) in
+    let res = NL.nlist_sorted
+      (jump_pair jump_raw_data_item jump_raw_data_item)
+      (map_entry_order_impl _ order_impl _)
+      n
+      _
+      ac
+    in
+    let _ = intro_raw_data_item_map a ac in
+    rewrite (aparse _ a _) (aparse (parse_recursive parse_raw_data_item_param) a va);
+    return res
+  end else begin
+    rewrite (aparse _ a _) (aparse (parse_recursive parse_raw_data_item_param) a va);
+    return true
+  end
+
+inline_for_extraction
+noextract
+let validate_data_item'
+  (#order: Ghost.erased (raw_data_item -> raw_data_item -> bool))
+  (order_impl: NL.order_impl parse_raw_data_item order)
+  (sq: squash (SZ.fits_u64))
+: Tot (validator (parse_data_item order))
+= rewrite_validator
+    (validate_filter_gen
+      validate_raw_data_item
+      (data_item_wf order)
+      (fun #va a ->
+        rewrite (aparse _ a _) (aparse (parse_recursive parse_raw_data_item_param) a va);
+        let res = pred_recursive
+          serialize_raw_data_item_param
+          (jump_leaf sq)
+          (jump_count_remaining_data_items sq)
+          a
+          (data_item_wf_pred order)
+          (check_data_item_wf_head order_impl sq)
+        in
+        rewrite (aparse _ a _) (aparse parse_raw_data_item a va);
+        return res
+      )
+    )
+    (parse_data_item order)
+
+#pop-options
+
+inline_for_extraction
+noextract
+let validate_data_item
+  (#order: Ghost.erased (raw_data_item -> raw_data_item -> bool))
+  (order_impl: NL.order_impl parse_raw_data_item order)
+: Tot (validator (parse_data_item order))
+= fun a len err ->
+    let sq = Steel.ST.HigherArray.intro_fits_u64 () in
+    validate_data_item' order_impl sq a len err
+
+let deterministically_encoded_cbor_map_key_order_impl
+: NL.order_impl parse_raw_data_item deterministically_encoded_cbor_map_key_order
+= fun #va1 #va2 a1 a2 ->
+    let n1 = get_parsed_size jump_raw_data_item a1 in
+    let n2 = get_parsed_size jump_raw_data_item a2 in
+    let vb1 = elim_aparse_with_serializer serialize_raw_data_item a1 in
+    let vb2 = elim_aparse_with_serializer serialize_raw_data_item a2 in
+    let res = LowParse.SteelST.SeqBytes.byte_array_lex_order n1 a1 n2 a2 in
+    let _ = intro_aparse parse_raw_data_item a1 in
+    let _ = intro_aparse parse_raw_data_item a2 in
+    vpattern_rewrite (aparse _ a1) va1;
+    vpattern_rewrite (aparse _ a2) va2;
+    return res
+
+let validate_deterministically_encoded_cbor_data_item
+: validator (parse_data_item deterministically_encoded_cbor_map_key_order)
+= validate_data_item deterministically_encoded_cbor_map_key_order_impl
+
+let canonical_cbor_map_key_order_impl
+: NL.order_impl parse_raw_data_item canonical_cbor_map_key_order
+= fun #va1 #va2 a1 a2 ->
+    let n1 = get_parsed_size jump_raw_data_item a1 in
+    let n2 = get_parsed_size jump_raw_data_item a2 in
+    let vb1 = elim_aparse_with_serializer serialize_raw_data_item a1 in
+    let vb2 = elim_aparse_with_serializer serialize_raw_data_item a2 in
+    let res = LowParse.SteelST.SeqBytes.byte_array_length_first_lex_order n1 a1 n2 a2 in
+    let _ = intro_aparse parse_raw_data_item a1 in
+    let _ = intro_aparse parse_raw_data_item a2 in
+    vpattern_rewrite (aparse _ a1) va1;
+    vpattern_rewrite (aparse _ a2) va2;
+    return res
+
+let validate_canonical_cbor_data_item
+: validator (parse_data_item canonical_cbor_map_key_order)
+= validate_data_item canonical_cbor_map_key_order_impl
+
+let jump_data_item
+  (order: Ghost.erased (raw_data_item -> raw_data_item -> bool))
+: Tot (jumper (parse_data_item order))
+= jump_filter
+    jump_raw_data_item
+    (data_item_wf order)
